\documentclass{report}

\usepackage{amsfonts}
\usepackage{amsmath}
\usepackage{amssymb}

\input{preamble}
\input{macros}
\input{letterfonts}

\title{\Huge{Analysis of Algorithms} \\ \huge{Homework 4}}

\author{\huge{Thomas Schollenberger (tss2344)}}
\date{}

\begin{document}

\maketitle

\qs{3}{
    The expected case time complexity for the select algorithm is characterized by the following recurrence \\
    \(T(1) = 2 \\
        T(n) = (n + 1) + \displaystyle\frac{1}{n}\displaystyle\sum_{q=1}^{n-1} T(q)
    \) \\
    Use techniques, including iteration, to solve the recurrence exactly.
}
\pf{Proof 3}{
    We know that:
    \begin{align*}
        T(n) &= (n + 1) + \displaystyle\frac{1}{n}\displaystyle\sum_{q=1}^{n-1} T(q) \\
        T(n + 1) &= (n + 2) + \displaystyle\frac{1}{n + 1}\displaystyle\sum_{q=1}^{n} T(q)
    \end{align*}
    From that definition, we can assert that:
    \begin{center}
        \(n\left(T(n) - (n + 1)\right) = \displaystyle\sum_{q=1}^{n-1} T(q)\)
    \end{center}
    Thus:
    \begin{align*}
        T(n + 1) - T(n) &= (n + 2) - (n + 1) + \left(\displaystyle\frac{1}{n + 1}\displaystyle\sum_{q=1}^{n} T(q) - \displaystyle\frac{1}{n}\displaystyle\sum_{q=1}^{n-1} T(q)\right) \\
        &= (n + 2) - (n + 1) + \left(\displaystyle\frac{1}{n + 1}\displaystyle\sum_{q=1}^{n-1} T(q) - \displaystyle\frac{1}{n}\displaystyle\sum_{q=1}^{n-1} T(q)\right) + \displaystyle\frac{1}{n+1}T(n) \\
        &= 1 + \left(\displaystyle\frac{1}{n + 1}\displaystyle\sum_{q=1}^{n-1} T(q) - \displaystyle\frac{1}{n}\displaystyle\sum_{q=1}^{n-1} T(q)\right) + \displaystyle\frac{1}{n+1}T(n) \\
        &= 1 + \left(\displaystyle\frac{1}{n + 1} - \displaystyle\frac{1}{n}\right) \displaystyle\sum_{q=1}^{n-1} T(q) + \displaystyle\frac{1}{n+1}T(n) \\
        &= 1 - \frac{1}{n\left(n+1\right)} \displaystyle\sum_{q=1}^{n-1} T(q) + \displaystyle\frac{1}{n+1}T(n)
    \end{align*}
    We can now substitute from the definition:
    \begin{align*}
        T(n + 1) - T(n) &= 1 - \frac{1}{n\left(n+1\right)} \left(n(T(n) - (n + 1)\right) + \displaystyle\frac{1}{n+1}T(n) \\
        &= 1 - \frac{T(n) - (n + 1)}{\left(n+1\right)} + \displaystyle\frac{T(n)}{n+1} \\
        &= 1 - \left(\displaystyle\frac{T(n)}{n+1} - 1\right) + \displaystyle\frac{T(n)}{n+1} \\
        &= 1 + \displaystyle\frac{-T(n)}{n+1} + 1 + \displaystyle\frac{T(n)}{n+1} \\
        &= 2
    \end{align*}
    Which means we end up with, after subtracting \(-T(n)\):
    \begin{align*}
        T(n + 1) &= T(n) + 2 \\
        &= 2n
    \end{align*}
    Proving that our select algorithm runs in \(\mathcal{O}(n)\) time
    
}
\end{document}
