\documentclass{article}

\usepackage{amsmath}
\usepackage{amssymb}
\usepackage[shortlabels]{enumitem}

\newcommand {\R}{\mathbb{R}}
\newcommand {\N}{\mathbb{N}}

\title{%
  Analysis of Algorithms \\
  \large Homework 1 }

\author{Thomas Schollenberger (tss2344)}

\begin{document}
\maketitle

\section*{Problem \#1}
Rank the following functions by order of growth. Further, partition the list into equivalence classes such that
functions \(f(n)\) and \(g(n)\) are in the same class iff \(f(n) \in \theta(g(n))\).
\begin{center}
\begin{tabular}{|c|c|c|c|c|}
    \hline
    \(\ln{(\ln{(x)}})\) & \(n2^n\) & \(n^{\lg{(\lg{(n)})}}\) & \(\ln{n}\) & \(1\) \\
    \hline
    \((\lg{(n)})^{\lg{(n)}}\) & \(e^n\) & \(4^{\lg{(n)}}\) & \((n + 1)!\) & \(\sqrt{\lg{(n)}}\) \\
    \hline
    \(n^3\) & \((\lg{(n)})^2\) & \(\lg{n!}\) & \(2^{2^{n}}\) & \(\frac{3}{2}^n\) \\
    \hline
    \(2^{\sqrt{2\lg{(n)}}}\) & \(n\) & \(2^{n}\) & \(n\lg{(n)}\) & \(2^{2^{n+1}}\) \\
    \hline
    \(2^{\lg{(n)}}\) & \(\sqrt{2}^{\lg{(n)}}\) & \(n^2\) & \(n!\) & \((\lg{(n)})!\) \\
    \hline
\end{tabular}
\end{center}
Equivalence Classes, where \(a \in \R\):
\[[\theta(1)] = \{1\},\]
\[[\theta(\sqrt{\lg{(x)}})] = \{\sqrt{\lg{(n)}}\},\]
\[[\theta(\ln{(x)})] = \{\ln{(\ln{(n)})}, ln{(n)}\},\]
\[[\theta(\lg{(x)})] = \{n\lg{(n)}, \lg{(n!)}\},\]
\[[\theta(x)] = \{n\},\]
\[[\theta(a^{\sqrt{n}})] = \{2^{\sqrt{2\lg{(n)}}}\},\]
\[[\theta(x^2)] = \{n^2, (\lg{(n)})^2\},\]
\[[\theta(x^3)] = \{n^3\},\]
\[[\theta(a^{\lg{(n)}})] = \{2^{\lg{(n)}}, \sqrt{2}^{\lg{(n)}}, (\lg{(n)})^{\lg{(n)}}, 4^{\lg{(n)}}\},\]
\[[\theta(n^{\lg{(n)}})] = \{n^{\lg{(\lg{(n)})}}\},\]
\[[\theta(a^n)] = \{n2^n, e^n, 2^n, \frac{3}{2}^n\},\]
\[[\theta(x!)] = \{(\lg{(n)})!, n!, (n + 1)!\}\]
\[[\theta(a^{a^x})] = \{2^{2^n}, 2^{2^{n+1}}\},\]
And the order of the functions, from highest to lowest, are:
\[2^{2^{n+1}}\]
\[2^{2^n}\]
\[(n+1)!\]
\[n!\]
\[e^{n}\]
\[n\left(2\right)^{n}\]
\[2^{n}\]
\[\frac{3}{2}^n\]
\[n^{\lg{(\lg{(n)})}}\]
\[(\lg{(n)})^{\lg{(n)}}\]
\[4^{\lg{(n)}}\]
\[\lg{(n)})!\]
\[n^3\]
\[n^2\]
\[n\lg{(n)}\]
\[\lg{(n!)}\]
\[2^{\lg{(n)}}, n \left(\text{These are functionally equivalent}\right)\]
\[\sqrt{2}^{\lg{(n)}}\]
\[2^{\sqrt{2\lg{(n)}}}\]
\[\lg{(n)}^2\]
\[ln{(n)}\]
\[\sqrt{\lg{(n)}}\]
\[\ln{(\ln{(n)})}\]
\[1\]

\section*{Problem \#2}
Let: \[a, b, c, k \in \R \]
We have the following functions: \[ \sqrt[k]{x}, a^x, x^c, \log_b{x} \]
We can translate them into: \[ x^\frac{1}{k}, a^x, x^c, \frac{\log{x}}{\log{b}} \]
For all constants, \(\lim_{x\to\infty}\): \[
    x^\frac{1}{k} < x^c,
    \frac{\log{x}}{\log{b}} < x^c,
    x^c < a^x,
    x^\frac{1}{k} < \frac{\log{x}}{\log{b}}
\]
Which gives us: \[ x^\frac{1}{k} < \frac{\log{x}}{\log{b}} < x^c < a^x \]

\section*{Problem \#3}
For all three proofs, consider:
\[ f(x) = n \implies f(x) \in \mathcal{O}(g(x)) \]
\[ N, c \in \R, N, c = 1 \]
\[ |f(x)| \leq c|g(x)| \]
\subsection*{a. Prove the following:}
Using the class definition of Big O, prove that \[ n = \mathcal{O}(n^2) \]
Suppose:
\[x \geq N \]
\[N \leq x \implies x \leq x^2 \]
\[x \leq x^2 \implies |x| \leq c|x^2| \]
Thus:
\[n = \mathcal{O}(n^2) \]
\subsection*{b. Prove the following:}
Using the class definition of Big O, prove that \[ n^2 = \mathcal{O}(n^2) \]
Suppose:
\[1 \geq 1 \]
\[1 \leq 1 \implies x \leq x \]
\[x \leq x \implies |x^2| \leq 1|x^2| \]
Thus:
\[n^2 = \mathcal{O}(n^2) \]
\subsection*{c. Prove the following:}
Using the class definition of Big O, prove that \[ 3n^2 + 5n = \mathcal{O}(n^2) \]
Suppose:
\[3x^2 + 5x \leq 3x^2 + 5x \]
\[3x^2 + 5x \leq 3x^2 + 5x^2 \]
\[3x^2 + 5x \leq 8x^2 \]
Thus:
\[N = 8, C = 1\]
\[|3x^2 + 5x| \leq 1|8x^2|\]
\[3x^2 + 5x = \mathcal{O}(x^2)\]

\section*{Project \#4}
Big \(\mathcal{O}\) proofs

\subsection*{a. Given that \(\sum_{k=2}^n \frac{1}{k} \leq \ln{(n)} - \ln{(1)}\), using the class definition of \(\mathcal{O}\), prove that \(H_n \in \mathcal{O}(\ln{(n)})\)}
Assuming \(1 \geq 1\), then:
\begin{align}
1 &\leq 1\\
n &\leq n\\
\ln{(n)} &\leq \ln{(n)}\\
\ln{(n)} - \ln{(1)} &\leq \ln{(n)} - \ln{(1)}\\
|\ln{(n)} - \ln{(1)}| &\leq 1|\ln{(n)}|
\end{align}
However, this only proves that \(H_2 \in \mathcal{O}(\ln{(n)})\). To prove \(H_1\), we need to add a one to each side:
\begin{align}
&\ln{(n)} - \ln{(1)} + 1 \leq \ln{(n)} + 1\\
&\ln{(n)} \leq \ln{(n)} - \ln{(1)} + 1 \leq \ln{(n)} + 1\\
&\ln{(n + 1)} \leq \ln{(n)} - \ln{(1)} \leq \ln{(n)}
\end{align}
Which shows that \(H_n \in \mathcal{O}(\ln{(n)})\)

\subsection*{b. Given that \(\sum_{k=2}^n \frac{1}{k} \geq \ln{(n + 1)} - \ln{(2)}\), using the class definition of \(\mathcal{\omega}\), prove that \(H_n \in \mathcal{\omega}(\ln{n})\)}
Assuming \(1 \leq 1\), then:
\begin{align}
1 &\geq 1\\
n &\geq n\\
\ln{(n)} &\geq \ln{(n)}\\
\ln{(n)} - \ln{(2)} &\geq \ln{(n)} - \ln{(2)}\\
|\ln{(n)} - \ln{(2)}| &\geq 1|\ln{(n)} - \ln{(2)}|
\end{align}
We then need to add + 1 to both sides:
\begin{align}
&|\ln{(n)} - \ln{(2)} + 1| \geq 1|\ln{(n)} - \ln{(2)} + 1|\\
&|\ln{(n)} - \ln{(2)} + 1| \geq 1|\ln{(n)} - \ln{(2)} + 1|\\
&|\ln{(n + 1)}| \geq |\ln{(n)} - \ln{(2)} + 1| \geq 1|\ln{(n)} - \ln{(2)} + 1|
\end{align}

Which then we can shift to
\[|\ln{(n)}| \geq |\ln{(n + 1)} - \ln{(2)}| \geq 1|\ln{(n + 1)} - \ln{(2)}|\]
Which shows that \(H_n \in \mathcal{\omega}(\ln{(n)})\)

\section*{Problem \#5}
The smallest \{n\} that fib starts slowing down at is 30.

\section*{Problem \#6}
Consider the following recurrence:
\[f(0; a, b) = a\]
\[f(1; a, b) = b\]
\[f(n; a, b) = f(n - 1; b, a + b)\]
\subsection*{a. Prove using mathematical induction that for any \(n \in \N\) if \(n > 1\) then \(f(n; a, b) = f(n - 1; a, b) + f(n - 2; a, b)\).}
% \[f(n; a, b) = f(n - 1; a, b) + f(n - 2; a, b)\]
Observe that, for \(n = 2\):
\begin{align}
f(2; a, b) &= f(1; b, a + b)\\
&= a + b\\
&= f(1; a, b) + f(0; a, b)\\
&= f(2 - 1; a, b) + f(2 - 2; a, b)
\end{align}

Assume that \(f(k; a, b) = f(k - 1; a, b) + f(k - 2; a, b)\) is true, where \(0 \leq k < n\), then:
\begin{align}
f(k + 1; a, b) &= f(k; b, a + b)\\
&= f(k - 1; b, a + b) + f(k - 2; b, a + b)\\
&= f(k; a, b) + f(k - 1; a, b)
\end{align}

Which proves f(n; a, b) = f(n - 1; a, b) + f(n - 2; a, b)
\subsection*{b. Prove using the strong form of induction that for any \(n \in \N, F_n = f(n; 0, 1)\). You should use the previous
result in your proof.}
Suppose \(F_2, F_3, ..., F_k \implies F_{k+1}\)
\[F_2 = f(2; 0, 1) = f(1; 0, 1) + f(0; 0, 1) = 1 + 0 = 1\]
\[F_3 = f(3; 0, 1) = f(2; 1, 1 + 0) = f(1; 1, 1 + 0 + 1) = 1 + 0 + 1 = 2\]
\[F_k = f(k - 1; 0, 1) + f(k - 2; 0, 1)\]
Assume that \(F_k = f(k - 1; 0, 1) + f(k - 2; 0, 1)\), then
\begin{align}
F_{k+1} &= f(k; 0, 1) + f(k - 1; 0, 1)\\
&= f(k + 1; 0, 1)
\end{align}
Which proves that for all n, \(F_n = f(n; 0, 1)\)
\section*{Problem \#7}
Exceeds maximum recursion depth before slowing down at all

\end{document}